

$$\int_0^1 x^5 e^{x^2} dx$$

# Learning Integration!

$$f(x) g'(x) \quad \int f(x) g'(x) = f(x) g(x) - \int f'(x) g(x) dx$$

$$\int_0^1 x^5 e^{x^2} dx$$

$$u = x^2 \quad du = 2x dx \quad dx = \frac{du}{2x}$$

$$x=0 \quad u=0 \quad x^5 = x \cdot x^4 = x \cdot u^2$$

$$x=1 \quad u=1$$

$$= \frac{1}{2} \int_0^1 x \cdot u^2 e^u \cdot \frac{du}{x} = \frac{1}{2} \int_0^1 u^2 e^u du = \frac{1}{2} \left( u^2 e^u \Big|_0^1 - 2 \int_0^1 u e^u du \right)$$

$$= \frac{1}{2} \left( u^2 e^u \Big|_0^1 - 2 \left( u e^u \Big|_0^1 - \int_0^1 e^u du \right) \right) = \frac{1}{2} \left( u e^u \Big|_0^1 - 2 u e^u \Big|_0^1 + 2 e^u \Big|_0^1 \right)$$

$$= \frac{1}{2} (e - 2/e + 2/e - 2) = \boxed{\frac{e}{2} - 1}$$

$$\sum_{k=0}^{\infty} \frac{x^k}{k!} = e^x \quad e^{x^2} = \sum_{k=0}^{\infty} \frac{x^{2k}}{k!}$$

$$I = \int_0^1 x^5 e^{x^2} dx = \int_0^1 x^5 \sum_{k=0}^{\infty} \frac{x^{2k}}{k!} dx = \sum_{k=0}^{\infty} \frac{1}{k!} \int_0^1 x^5 \cdot x^{2k} dx$$

$$= I = \sum_{k=0}^{\infty} \frac{1}{k!} \int_0^1 x^{5+2k} dx = \sum_{k=0}^{\infty} \frac{1}{k!} \cdot \frac{x^{6+2k}}{6+2k} \Big|_0^1$$

$$= \sum_{k=0}^{\infty} \frac{1}{k!} \cdot \frac{1}{6+2k} = \frac{1}{2} \sum_{k=0}^{\infty} \frac{1}{k! (3+k)}$$

$$(k+3)! = (k+3)(k+2)(k+1)k! \quad k! = \frac{(k+3)!}{(k+1)(k+2)(k+3)}$$

$$= \frac{1}{2} \sum_{k=0}^{\infty} \frac{1}{(k+3)!} \cdot (k+1)(k+2)$$

$$= \frac{1}{2} \sum_{k=0}^{\infty} \frac{(k+1)(k+2)}{(k+3)!} = \frac{k^2 + 3k + 2}{(k+3)!}$$

$$= \frac{(k+3)^2 - 3(k+3) + 2}{(k+3)!} = \frac{(k+3)^2}{(k+3)!} - \frac{3(k+3)}{(k+3)!} + \frac{2}{(k+3)!}$$

$$(1) \quad \frac{(k+3)(k+3)}{(k+3)(k+2)!} = \frac{(k+3)+1}{(k+2)!(k+2)!} = \frac{k+2}{(k+2)(k+1)!} + \frac{1}{(k+2)!}$$

$$(2) \quad \frac{-3(k+3)}{(k+3)(k+2)!} = \frac{-3}{(k+2)!} \quad (3) \quad \frac{2}{(k+3)!}$$

$$\frac{1}{(k+1)!} - \frac{2}{(k+2)!} + \frac{2}{(k+3)!}$$

$$\sum_{k=0}^{\infty} \frac{1}{(k+1)!} - \sum_{k=0}^{\infty} \frac{2}{(k+2)!} + 2 \sum_{k=0}^{\infty} \frac{1}{(k+3)!}$$

$$\sum_{k=1}^{\infty} \frac{1}{k!} = e - 1 \quad 2 \sum_{k=2}^{\infty} \frac{1}{k!} = -2(e - 1 - 1) = -2e + 4$$

$$2 \sum_{k=3}^{\infty} \frac{1}{k!} = e - 1 - 1 - \frac{1}{2} = 2e - 2\frac{1}{2} = 2e - \frac{5}{2}$$







